broken but sharing

src/SourceLang.v
@@ -7,6 +7,7 @@ Require Import HList.
 
 Require Import Utopia.
 
+
 Inductive type :=
 | ADT : type_name -> type
 | Arrow : type -> type -> type
@@ -1266,3 +1267,15 @@ Proof.
   eapply Eqdep_dec.inj_pair2_eq_dec in H3; try eapply list_eq_dec; try eapply type_eq_dec; try decide equality.
   congruence.
 Defined.
+(*
+Require Semantics.
+
+Definition Semantics {ty} (exp : expr [] ty) : Semantics.semantics.
+  refine (Semantics.Semantics_gen _ _ _ _ _ _ _).
+  exact (fun x : unit => (@step [] ty)).
+  admit.
+  admit.
+  exact tt.
+  repeat (econstructor; eauto); admit.
+Admitted.
+*)
