src/UntypedComp.v
@@ -26,6 +26,7 @@ Definition elim_to_type_name {l cases target} (e : S.elim l cases target) : type
   | S.EPositive _ => Tpositive
   end.
 
+
 Definition compile {l ty} (e : S.expr l ty) : U.expr :=
   let fix go {l ty} (e : S.expr l ty) : U.expr :=
       let fix go_hlist {l tys} (h : hlist (S.expr l) tys) : list U.expr :=
